Transformers/Locality.thy
@@ -141,6 +141,8 @@ proof -
   finally show ?thesis
     apply simp
     apply default
+    sorry
+qed
 
 
 
